Makefile
@@ -115,6 +115,8 @@ ROOT_FILES = \
   src/impl/TLS13.System.ServerNotCFR.fst \
   src/impl/TLS13.System.AppBothCongruence.fst \
   src/impl/TLS13.System.AppMaterialFamilies.fst \
+  src/impl/TLS13.System.AppExtrasInv.fst \
+  src/impl/TLS13.System.HsSeqPairing.fst \
   src/spec/properties/TLS13.ConnectionState.HandshakeAgreementNonReady.fst \
   src/spec/properties/TLS13.ConnectionState.ServerHelloSelectionLink.fst \
   src/spec/properties/TLS13.ConnectionState.HandshakeSeqZero.fst \
